ironfleet/src/Dafny/Distributed/Protocol/Lock/PerformanceProof/PerformanceProof.i.dfy
@@ -10,7 +10,7 @@ import opened LockTaggedDistributedSystem_i
   import opened PerformanceProof__Definitions_i
   import opened Math__mod_auto_i
 
-predicate {:verify false} SingleGLSPerformanceAssumption(tgls:TaggedGLS_State)
+predicate SingleGLSPerformanceAssumption(tgls:TaggedGLS_State)
 {
   // The only nodes that take steps are in the ring
   && (tgls.tls.t_environment.nextStep.LEnvStepHostIos? ==> tgls.tls.t_environment.nextStep.actor in tgls.tls.t_servers)
@@ -29,31 +29,31 @@ predicate {:verify false} SingleGLSPerformanceAssumption(tgls:TaggedGLS_State)
 
 }
 
-predicate {:verify false} GLSPerformanceAssumption(tglb:seq<TaggedGLS_State>)
+predicate GLSPerformanceAssumption(tglb:seq<TaggedGLS_State>)
 {
   forall tgls :: tgls in tglb ==> SingleGLSPerformanceAssumption(tgls)
 }
 
-predicate {:verify false} SingleGLSPerformanceGuarantee(gls:TaggedGLS_State)
+predicate SingleGLSPerformanceGuarantee(gls:TaggedGLS_State)
 {
   |gls.tls.config| > 1 ==> 
   (forall pkt :: pkt in gls.tls.t_environment.sentPackets &&
     pkt.msg.v == Transfer(|gls.tls.config|) ==> PerfEq(pkt.msg.pr, PerfBoundLockInNetwork(|gls.tls.config|)))
 }
 
-predicate {:verify false} GLSPerformanceGuarantee(tglb:seq<TaggedGLS_State>)
+predicate GLSPerformanceGuarantee(tglb:seq<TaggedGLS_State>)
 {
   forall tgls :: tgls in tglb ==> SingleGLSPerformanceGuarantee(tgls)
 }
 
-predicate {:verify false} TGLS_Consistency(tgls: TaggedGLS_State)
+predicate TGLS_Consistency(tgls: TaggedGLS_State)
 {
   && (forall id :: id in tgls.tls.config <==> id in tgls.tls.t_servers)
     && (forall id :: id in tgls.tls.t_servers ==> (tgls.tls.t_servers[id].v.config == tgls.tls.config))
     && (forall i :: 0 <= i < |tgls.tls.config| ==> tgls.tls.t_servers[tgls.tls.config[i]].v.my_index == i)
 }
 
-predicate {:verify false} PerfInvariantAlways(tgls:TaggedGLS_State)
+predicate PerfInvariantAlways(tgls:TaggedGLS_State)
   requires TGLS_Consistency(tgls)
 {
   // No irrelevant packets in sentPackets
@@ -73,7 +73,7 @@ predicate {:verify false} PerfInvariantAlways(tgls:TaggedGLS_State)
   ==> 0 < pkt.msg.v.locked_epoch <= |tgls.history|)
 }
 
-predicate {:verify false} PerfInvariantLockHeld(tgls: TaggedGLS_State, j:int, epoch:int)
+predicate PerfInvariantLockHeld(tgls: TaggedGLS_State, j:int, epoch:int)
   requires 0 < epoch
   requires 0 <= j < |tgls.tls.config|
   requires TGLS_Consistency(tgls)
@@ -109,7 +109,7 @@ predicate {:verify false} PerfInvariantLockHeld(tgls: TaggedGLS_State, j:int, ep
   )
 }
 
-predicate {:verify false} PerfInvariantLockInNetwork(tgls: TaggedGLS_State, j:int, epoch:int)
+predicate PerfInvariantLockInNetwork(tgls: TaggedGLS_State, j:int, epoch:int)
   requires 1 < epoch
   requires 0 < j < |tgls.tls.config|
   requires TGLS_Consistency(tgls)
@@ -149,7 +149,7 @@ predicate {:verify false} PerfInvariantLockInNetwork(tgls: TaggedGLS_State, j:in
   )
 }
 
-predicate {:verify false} PerfInvariantEpochHigherThanNumServers(tgls:TaggedGLS_State)
+predicate PerfInvariantEpochHigherThanNumServers(tgls:TaggedGLS_State)
   requires TGLS_Consistency(tgls)
 {
   && PerfInvariantAlways(tgls)
@@ -165,7 +165,7 @@ predicate {:verify false} PerfInvariantEpochHigherThanNumServers(tgls:TaggedGLS_
 }
 
 // TODO: Change this invariant
-predicate {:verify false} PerfInvariantNodeZeroGrantedLock(tgls:TaggedGLS_State)
+predicate PerfInvariantNodeZeroGrantedLock(tgls:TaggedGLS_State)
   requires 0 < |tgls.tls.config|
   requires TGLS_Consistency(tgls)
 {
@@ -175,7 +175,7 @@ predicate {:verify false} PerfInvariantNodeZeroGrantedLock(tgls:TaggedGLS_State)
     && tgls.tls.t_servers[tgls.tls.config[0]].v.epoch == |tgls.history|
 }
 
-predicate {:verify false} PerfInvariantNodeZeroReceivedLock(tgls:TaggedGLS_State)
+predicate PerfInvariantNodeZeroReceivedLock(tgls:TaggedGLS_State)
   requires TGLS_Consistency(tgls)
 {
   && 0 < |tgls.tls.config|
@@ -185,7 +185,7 @@ predicate {:verify false} PerfInvariantNodeZeroReceivedLock(tgls:TaggedGLS_State
     && tgls.tls.t_servers[tgls.tls.config[0]].v.epoch == |tgls.history|
 }
 
-lemma {:verify false} NotHostIos_InvLockHeldImpliesInvLockHeld(j:int, epoch:int, s:TaggedGLS_State, s':TaggedGLS_State)
+lemma NotHostIos_InvLockHeldImpliesInvLockHeld(j:int, epoch:int, s:TaggedGLS_State, s':TaggedGLS_State)
   requires TGLS_Next(s, s')
   requires 0 <= j < |s.tls.config|
   requires 0 < epoch
@@ -200,7 +200,7 @@ lemma {:verify false} NotHostIos_InvLockHeldImpliesInvLockHeld(j:int, epoch:int,
   //reveal_PerfInvariantLockHeld();
 }
 
-lemma {:verify false} Grant_not_j_InvLockHeldImpliesInvLockHeld(j:int, epoch:int, s:TaggedGLS_State, s':TaggedGLS_State)
+lemma Grant_not_j_InvLockHeldImpliesInvLockHeld(j:int, epoch:int, s:TaggedGLS_State, s':TaggedGLS_State)
   requires TGLS_Next(s, s')
   requires 0 <= j < |s.tls.config|
   requires 0 < epoch <= |s.tls.config|
@@ -219,7 +219,7 @@ lemma {:verify false} Grant_not_j_InvLockHeldImpliesInvLockHeld(j:int, epoch:int
   //reveal_PerfInvariantLockHeld();
 }
 
-lemma {:verify false} Accept_not_j_InvLockHeldImpliesInvLockHeld(j:int, epoch:int, s:TaggedGLS_State, s':TaggedGLS_State)
+lemma Accept_not_j_InvLockHeldImpliesInvLockHeld(j:int, epoch:int, s:TaggedGLS_State, s':TaggedGLS_State)
   requires TGLS_Next(s, s')
   requires 0 <= j < |s.tls.config|
   requires 0 < epoch <= |s.tls.config|
@@ -235,10 +235,11 @@ lemma {:verify false} Accept_not_j_InvLockHeldImpliesInvLockHeld(j:int, epoch:in
   ensures PerfInvariantLockHeld(s', j, epoch);
 {
   lemma_mod_auto(|s.tls.config|);
-  //reveal_PerfInvariantLockHeld();
+  var ios := s.tls.t_environment.nextStep.ios;
+  assert IsValidLIoOp(ios[0], s.tls.t_environment.nextStep.actor, s.tls.t_environment);
 }
 
-lemma {:verify false} Grant_j_InvLockHeldImpliesInvLockInNetwork(j:int, epoch:int, s:TaggedGLS_State, s':TaggedGLS_State)
+lemma Grant_j_InvLockHeldImpliesInvLockInNetwork(j:int, epoch:int, s:TaggedGLS_State, s':TaggedGLS_State)
   requires TGLS_Next(s, s')
   requires 0 <= j < |s.tls.config| - 1
   requires 0 < epoch < |s.tls.config|
@@ -258,13 +259,14 @@ lemma {:verify false} Grant_j_InvLockHeldImpliesInvLockInNetwork(j:int, epoch:in
   //reveal_PerfInvariantLockInNetwork();
 
   lemma_mod_auto(|s.tls.config|);
-  PerfProperties();
+  // PerfProperties();
   //var p := PerfBoundLockHeld(epoch);
   //var p' := PerfBoundLockInNetwork(epoch + 1);
   //assert PerfEq(p', PerfAdd2(p, PerfStep(GrantStep)));
+  Grant_j_helper_specific(epoch);
 }
 
-lemma {:verify false} Grant_LastNode_InvLockHeldImpliesInvEpochHigher(j:int, epoch:int, s:TaggedGLS_State, s':TaggedGLS_State)
+lemma Grant_LastNode_InvLockHeldImpliesInvEpochHigher(j:int, epoch:int, s:TaggedGLS_State, s':TaggedGLS_State)
   requires TGLS_Next(s, s')
   requires 0 <= j == |s.tls.config| - 1
   requires 0 <= epoch == |s.tls.config|
@@ -284,13 +286,13 @@ lemma {:verify false} Grant_LastNode_InvLockHeldImpliesInvEpochHigher(j:int, epo
   //reveal_PerfInvariantLockInNetwork();
 
   lemma_mod_auto(|s.tls.config|);
-  PerfProperties();
+  // PerfProperties();
   var p := PerfBoundLockHeld(epoch);
   var p' := PerfBoundLockInNetwork(epoch + 1);
-  assert PerfEq(p', PerfAdd2(p, PerfStep(GrantStep)));
+  // assert PerfEq(p', PerfAdd2(p, PerfStep(GrantStep)));
 }
 
-lemma {:verify false} NotHostIos_InvLockInNetworkImpliesInvLockInNetwork(j:int, epoch:int, s:TaggedGLS_State, s':TaggedGLS_State)
+lemma NotHostIos_InvLockInNetworkImpliesInvLockInNetwork(j:int, epoch:int, s:TaggedGLS_State, s':TaggedGLS_State)
   requires TGLS_Next(s, s')
   requires 0 < j < |s.tls.config|
   requires 1 < epoch <= |s.tls.config|
@@ -305,7 +307,7 @@ lemma {:verify false} NotHostIos_InvLockInNetworkImpliesInvLockInNetwork(j:int, 
   //reveal_PerfInvariantLockInNetwork();
 }
 
-lemma {:verify false} Accept_not_j_InvLockInNetworkImpliesInvLockInNetwork(j:int, epoch:int, s:TaggedGLS_State, s':TaggedGLS_State)
+lemma Accept_not_j_InvLockInNetworkImpliesInvLockInNetwork(j:int, epoch:int, s:TaggedGLS_State, s':TaggedGLS_State)
   requires TGLS_Next(s, s')
   requires 0 < j < |s.tls.config|
   requires 1 < epoch <= |s.tls.config|
@@ -322,7 +324,7 @@ lemma {:verify false} Accept_not_j_InvLockInNetworkImpliesInvLockInNetwork(j:int
   ensures PerfInvariantLockInNetwork(s', j, epoch);
 {
   //reveal_PerfInvariantLockInNetwork();
-
+  assert s.tls.t_environment.nextStep.ios[0] in s.tls.t_environment.nextStep.ios;
   lemma_mod_auto(|s.tls.config|);
 }
 
@@ -347,10 +349,11 @@ lemma Accept_j_InvLockInNetworkImpliesInvLockHeld(j:int, epoch:int, s:TaggedGLS_
   // PerfProperties();
   lemma_mod_auto(|s.tls.config|);
   assert s.tls.t_environment.nextStep.ios[0] in s.tls.t_environment.nextStep.ios;
-  lemma_Accept_j_PR(s.tls.t_environment.nextStep.ios[0].r.msg.pr, s.tls.t_servers[s.tls.config[j]].pr, s'.tls.t_servers[s.tls.config[j]].pr, epoch);
+  Accept_j_helper();
+  // lemma_Accept_j_PR(s.tls.t_environment.nextStep.ios[0].r.msg.pr, s.tls.t_servers[s.tls.config[j]].pr, s'.tls.t_servers[s.tls.config[j]].pr, epoch);
 }
 
-lemma {:verify false} PerfInvariantLockInNetworkGoesToPerfInvariant(j:int, epoch:int, s:TaggedGLS_State, s':TaggedGLS_State)
+lemma PerfInvariantLockInNetworkGoesToPerfInvariant(j:int, epoch:int, s:TaggedGLS_State, s':TaggedGLS_State)
   requires SingleGLSPerformanceAssumption(s) && TGLS_Consistency(s)
   requires SingleGLSPerformanceAssumption(s') && TGLS_Consistency(s')
   requires TGLS_Next(s, s')
@@ -384,7 +387,7 @@ lemma {:verify false} PerfInvariantLockInNetworkGoesToPerfInvariant(j:int, epoch
 
 ////////////////////////////////////////////////////////////////////////////////
 
-predicate {:verify false} PerfInvariant(tgls:TaggedGLS_State)
+predicate PerfInvariant(tgls:TaggedGLS_State)
 {
   && TGLS_Consistency(tgls)
   && ( 
@@ -394,7 +397,7 @@ predicate {:verify false} PerfInvariant(tgls:TaggedGLS_State)
   )
 }
 
-lemma {:verify false} NotHostIos_InvEpochHigherGoesToInvEpochHigher(j:int, s:TaggedGLS_State, s':TaggedGLS_State)
+lemma NotHostIos_InvEpochHigherGoesToInvEpochHigher(j:int, s:TaggedGLS_State, s':TaggedGLS_State)
   requires TGLS_Next(s, s')
   requires 0 <= j < |s.tls.config|
   requires TGLS_Consistency(s) && TGLS_Consistency(s')
@@ -409,7 +412,7 @@ lemma {:verify false} NotHostIos_InvEpochHigherGoesToInvEpochHigher(j:int, s:Tag
   lemma_mod_auto(|s.tls.config|);
 }
 
-lemma {:verify false} Grant_j_InvEpochHigherGoesToInvEpochHigher(j:int, s:TaggedGLS_State, s':TaggedGLS_State)
+lemma Grant_j_InvEpochHigherGoesToInvEpochHigher(j:int, s:TaggedGLS_State, s':TaggedGLS_State)
   requires TGLS_Next(s, s')
   requires 0 <= j < |s.tls.config|
   requires TGLS_Consistency(s) && TGLS_Consistency(s')
@@ -426,7 +429,7 @@ lemma {:verify false} Grant_j_InvEpochHigherGoesToInvEpochHigher(j:int, s:Tagged
   lemma_mod_auto(|s.tls.config|);
 }
 
-lemma {:verify false} PerfInvariantEpochHigherGoesToPerfInvariant(s:TaggedGLS_State, s':TaggedGLS_State)
+lemma PerfInvariantEpochHigherGoesToPerfInvariant(s:TaggedGLS_State, s':TaggedGLS_State)
   requires SingleGLSPerformanceAssumption(s) && TGLS_Consistency(s)
   requires SingleGLSPerformanceAssumption(s') && TGLS_Consistency(s')
   requires TGLS_Next(s, s')
@@ -447,7 +450,7 @@ lemma {:verify false} PerfInvariantEpochHigherGoesToPerfInvariant(s:TaggedGLS_St
   }
 }
 
-lemma {:verify false} PerfInvariantLockHeldGoesToPerfInvariant(j:int, epoch:int, s:TaggedGLS_State, s':TaggedGLS_State)
+lemma PerfInvariantLockHeldGoesToPerfInvariant(j:int, epoch:int, s:TaggedGLS_State, s':TaggedGLS_State)
   requires SingleGLSPerformanceAssumption(s) && TGLS_Consistency(s)
   requires SingleGLSPerformanceAssumption(s') && TGLS_Consistency(s')
   requires TGLS_Next(s, s')
@@ -482,7 +485,7 @@ lemma {:verify false} PerfInvariantLockHeldGoesToPerfInvariant(j:int, epoch:int,
   }
 }
 
-lemma {:verify false} PerfInvariantMaintained(s:TaggedGLS_State, s':TaggedGLS_State)
+lemma PerfInvariantMaintained(s:TaggedGLS_State, s':TaggedGLS_State)
   requires SingleGLSPerformanceAssumption(s) && TGLS_Consistency(s)
   requires SingleGLSPerformanceAssumption(s') && TGLS_Consistency(s')
   requires TGLS_Next(s, s')
@@ -503,7 +506,7 @@ lemma {:verify false} PerfInvariantMaintained(s:TaggedGLS_State, s':TaggedGLS_St
   }
 }
 
-lemma {:verify false} Establish_TGLS_Consistency(config:Config, tglb:seq<TaggedGLS_State>, i:int)
+lemma Establish_TGLS_Consistency(config:Config, tglb:seq<TaggedGLS_State>, i:int)
   requires ValidTaggedGLSBehavior(tglb, config)
   requires 0 <= i < |tglb|
   ensures TGLS_Consistency(tglb[i])
@@ -515,17 +518,17 @@ lemma {:verify false} Establish_TGLS_Consistency(config:Config, tglb:seq<TaggedG
   }
 }
 
-lemma {:verify false} InitImpliesPerfInvariant(config:Config, s:TaggedGLS_State)
+lemma InitImpliesPerfInvariant(config:Config, s:TaggedGLS_State)
   requires TGLS_Init(s, config)
   requires TGLS_Consistency(s);
   ensures PerfInvariant(s)
 {
   //reveal_PerfInvariantLockHeld();
-  PerfProperties();
+  // PerfProperties();
   assert PerfInvariantLockHeld(s, 0, 1);
 }
 
-lemma {:verify false} PerfInvariantImpliesPerfGuarantee(s:TaggedGLS_State)
+lemma PerfInvariantImpliesPerfGuarantee(s:TaggedGLS_State)
   requires PerfInvariant(s)
   ensures SingleGLSPerformanceGuarantee(s)
 {
@@ -533,7 +536,7 @@ lemma {:verify false} PerfInvariantImpliesPerfGuarantee(s:TaggedGLS_State)
   //reveal_PerfInvariantLockInNetwork();
 }
 
-lemma {:verify false} PerformanceGuaranteeHolds(config:Config, tglb:seq<TaggedGLS_State>)
+lemma PerformanceGuaranteeHolds(config:Config, tglb:seq<TaggedGLS_State>)
   requires ValidTaggedGLSBehavior(tglb, config)
   requires GLSPerformanceAssumption(tglb)
   ensures GLSPerformanceGuarantee(tglb)
